dll remove verified? -- needed props are much fewer than I expected?

SlowTest/DLL-ADT-short.dfy
@@ -2,125 +2,323 @@ newtype{:nativeType "ulong"} uint64 = i:int | 0 <= i < 0x1_0000_0000_0000_0000
 
 datatype Option<V> = None | Some(value:V) 
 type AbInt(==)
-function method int2adt (n: int) : (r: AbInt)
-predicate AbIsZero (n: AbInt) {n == int2adt(0)}
-predicate AbNonNeg (n: AbInt) { true }
-predicate AbPos (n: AbInt) {AbNonNeg(n) && !AbIsZero(n)}
-
+const I0 : AbInt := int2adt(0)
+const I1 : AbInt := int2adt(1)
+function method int2adt (n: int) : AbInt
+predicate AbIsZero (n: AbInt) { n == I0 }
+predicate AbPos (n: AbInt) { AbLt(I0, n) }
 function method AbLt(n: AbInt, m: AbInt) : bool
-function method AbAdd(n: AbInt, m: AbInt) : (r: AbInt)
-function method AbSub(n: AbInt, m: AbInt) : (r: AbInt)
-lemma Props_plus_and_minus ()
-  ensures forall x, y, z :: AbAdd(x, y) == z ==> AbSub(z, y) == x && AbSub(z, x) == y
+function method AbAdd(n: AbInt, m: AbInt) : AbInt
+function method AbSub(n: AbInt, m: AbInt) : AbInt
 
-function method seq_get<A>(s:seq<A>, i:uint64):(a:A)
-  requires i as int < |s|
-  ensures a == s[i] 
+lemma Props_int_pos(a: int)
+  ensures AbPos(int2adt(a))
+lemma Props_ltgteq () // x < y or x > y or x == y
+  ensures forall x, y :: AbLt(x, y) || AbLt(y, x) || x == y
+  ensures forall x, y :: AbLt(x, y) ==> x != y
 
-function method seq_set<A>(s1:seq<A>, i:uint64, a:A):(s2:seq<A>) // can be implemented as in-place update
-  requires i as nat < |s1|
-  ensures s2 == s1[i as nat := a] 
+lemma Props_lt_addition () // a < b ==> x + a < x + b
+  ensures forall x, a, b:: AbLt(a, b) ==> AbLt(AbAdd(x, a), AbAdd(x, b))
+  ensures forall x, a, b:: AbLt(a, b) ==> AbLt(AbSub(a, x), AbSub(b, x))
+lemma Props_lt_transitive () // x < y < z
+  ensures forall x, y, z :: AbLt(x, y) && AbLt(y, z) ==> AbLt(x, z)
+lemma Props_lt_transitive_xy (x: AbInt, y: AbInt) // x < y < z
+  ensures forall z :: AbLt(x, y) && AbLt(y, z) ==> AbLt(x, z)
+lemma Props_lt_transitive_z (z: AbInt) // x < y < z
+  ensures forall x, y :: AbLt(x, y) && AbLt(y, z) ==> AbLt(x, z)
+lemma Props_gt2geq ()
+  ensures forall x, y :: AbLt(x, y) <==> AbLt(AbAdd(x, I1), y) || AbAdd(x, I1) == y
+  ensures forall x, y :: AbLt(x, y) <==> AbLt(x, AbSub(y, I1)) || x == AbSub(y, I1)
+lemma Props_gt2geq_p1 (x: AbInt)
+  ensures forall y :: AbLt(x, y) <==> AbLt(AbAdd(x, I1), y) || AbAdd(x, I1) == y
+  ensures forall y :: AbLt(x, y) <==> AbLt(x, AbSub(y, I1)) || x == AbSub(y, I1)
 
-datatype Node<A> = Node(data:Option<A>, next:uint64, prev:uint64)
+lemma Props_add2sub () // x + y == z ==> x = z - y && y = z - x
+  ensures forall x, y, z :: AbAdd(x, y) == z <==> AbSub(z, y) == x
+  ensures forall x, y, z :: AbAdd(x, y) == z <==> AbSub(z, x) == y
+  ensures forall x, y :: AbAdd(AbSub(x, y), y) == x
+  ensures forall x, y :: AbSub(AbAdd(x, y), y) == x
+lemma Props_add_pos_is_lt () // x < x + Positive
+  ensures forall x, a :: AbPos(a) ==> AbLt(x, AbAdd(x, a));
+
+type AbSeq<X>
+function method AbSeqLen<X> (s: AbSeq<X>) : AbInt
+function method AbSeqIndex<X> (i: AbInt, s: AbSeq<X>) : X
+  requires AbLt(I0, i) || i == I0
+  requires AbLt(i, AbSeqLen(s))
+  ensures AbSeqIn(AbSeqIndex(i, s), s)
+
+function method AbSeqConcat<X> (s1: AbSeq<X>, s2: AbSeq<X>) : AbSeq<X>
+function method AbSeqIn<X> (v: X, s: AbSeq<X>) : bool
+
+function method AbSeqEmpty<X> (): (s: AbSeq<X>)
+  ensures AbSeqLen(s) == I0
+
+function method AbSeqSingleton<X(!new)> (v: X): (s: AbSeq<X>)
+  ensures AbSeqLen(s) == I1
+  ensures AbLt(I0, I1) ==> AbSeqIndex(I0, s) == v
+  ensures AbSeqIn(v, s)
+  ensures forall x :: x != v ==> !AbSeqIn(x, s)
+
+function method AbSeqSlice<X> (i: AbInt, j: AbInt, s: AbSeq<X>) : (s' : AbSeq<X>)
+  requires AbLt(I0, i) || i == I0
+  requires AbLt(j, AbSeqLen(s)) || j == AbSeqLen(s)
+  requires AbLt(i, j) || i == j
+  ensures AbSeqLen(s') == AbSub(j, i)
+  // Props_lt_transitive ();
+  ensures forall x :: AbLt(x, j) ==> AbLt(x, AbSeqLen(s))
+  ensures forall x :: (AbLt(i, x) || i == x) ==> (AbLt(I0, x) || x == I0)
+  // Props_add2sub (); Props_lt_addition ();
+  ensures forall x, y :: AbLt(x, y) ==> AbLt(AbSub(x, i), AbSub(y, i))
+  ensures forall x :: (AbLt(i, x) || i == x) ==> (AbLt(I0, AbSub(x, i)) || AbSub(x, i) == I0)
+  ensures forall x :: (AbLt(i, x) || i == x) && AbLt(x, j) ==> 
+    AbSeqIndex(x, s) == 
+    AbSeqIndex(AbSub(x, i), s') // s[i..j] w/ s[i] and w/o s[j]
+
+function method AbSeqGetIdx<X>(v: X, s: AbSeq<X>) : (i: AbInt)
+  requires AbSeqIn(v, s)
+  ensures AbLt(I0, i) || i == I0
+  ensures AbLt(i, AbSeqLen(s))
+  ensures AbSeqIndex(i, s) == v
+
+lemma Seq_Props_index_props<X> ()
+  ensures forall i: AbInt, x: AbInt, s: AbSeq<X> :: ((AbLt(I0, i) || I0 == i) && AbLt(i, AbSeqLen(s)) && AbLt(x, i)) ==> (forall j: AbInt :: (AbLt(I0, AbAdd(i, j)) || I0 == AbAdd(i, j)) && AbLt(AbAdd(i, j), AbSeqLen(s)) && AbLt(x, AbAdd(i, j)))
+  ensures forall i: AbInt, x: AbInt, s: AbSeq<X> :: ((AbLt(I0, i) || I0 == i) && AbLt(i, AbSeqLen(s)) && AbLt(i, x)) ==> (forall j: AbInt :: (AbLt(I0, AbAdd(i, j)) || I0 == AbAdd(i, j)) && AbLt(AbAdd(i, j), AbSeqLen(s)) && AbLt(AbAdd(i, j), x))
+lemma Seq_Props_index_props_jxs<X> (j: AbInt, x: AbInt, s: AbSeq<X>)
+  ensures forall i: AbInt :: ((AbLt(I0, i) || I0 == i) && AbLt(i, AbSeqLen(s)) && AbLt(x, i)) ==> ((AbLt(I0, AbAdd(i, j)) || I0 == AbAdd(i, j)) && AbLt(AbAdd(i, j), AbSeqLen(s)) && AbLt(x, AbAdd(i, j)))
+  ensures forall i: AbInt :: ((AbLt(I0, i) || I0 == i) && AbLt(i, AbSeqLen(s)) && AbLt(i, x)) ==> ((AbLt(I0, AbAdd(i, j)) || I0 == AbAdd(i, j)) && AbLt(AbAdd(i, j), AbSeqLen(s)) && AbLt(AbAdd(i, j), x))
+
+datatype Node<A> = Node(data:Option<A>, next:AbInt, prev:AbInt)
 datatype DList<A> = DList(
-  nodes:seq<Node<A>>, // sequence of nodes held by the list, indexed by pointer p
-  freeStack:uint64, // pointer to singly-linked stack of free nodes
-  ghost s:seq<A>, // sequence of data values held by the list, indexed by integer index i
-  ghost f:seq<int>, // map index to pointer: f[i] = p (where p > 0)
-  ghost g:seq<int>  // map pointer to index: g[p] = i (where g[p] == -2 means p is unused and g[0] == -1 (sentinel))
+  nodes:AbSeq<Node<A>>, // sequence of nodes held by the list, indexed by pointer p
+  freeStack:AbInt, // pointer to singly-linked stack of free nodes
+  ghost s:AbSeq<A>, // sequence of data values held by the list, indexed by integer index i
+  ghost f:AbSeq<AbInt>, // map index to pointer: f[i] = p (where p > 0)
+  ghost g:AbSeq<AbInt>  // map pointer to index: g[p] = i (where g[p] == -2 means p is unused and g[0] == -1 (sentinel))
   )
 
-ghost const unused:int := -2
-ghost const sentinel:int := -1
+ghost const unused: AbInt := AbSub(AbSub(I0, I1), I1) // -2
+ghost const sentinel: AbInt := AbSub(I0, I1)// -1
 
 // make sure the list-seq mapping is correct.
-predicate Invs<A>(nodes:seq<Node<A>>, freeStack:uint64, s:seq<A>, f:seq<int>, g:seq<int>)
+predicate Invs<A>(nodes:AbSeq<Node<A>>, freeStack:AbInt, s:AbSeq<A>, f:AbSeq<AbInt>, g:AbSeq<AbInt>)
 {
-  && |f| == |s|
-  && |g| == |nodes|
-  && |nodes| > 0
-  && g[0] == sentinel
-  && 0 <= freeStack as int < |nodes|
-  && (forall i :: 0 <= i < |f| ==> 0 < f[i] < |nodes|)
-  && (forall i {:trigger g[f[i]]} :: 0 <= i < |f| ==> g[f[i]] == i)
-  && (forall p :: 0 <= p < |g| ==>
-    && unused <= g[p] < |s|
-    && 0 <= nodes[p].next as int < |g|
-    && (g[p] >= 0 <==> nodes[p].data.Some?))
-  && (forall p :: 0 <= p < |g| && sentinel <= g[p] ==>
-    && (g[p] == sentinel ==> p == 0)
-    && (0 <= g[p] ==> f[g[p]] == p && nodes[p].data == Some(s[g[p]]))
-    && nodes[p].next as int == (
-      if g[p] + 1 < |f| then f[g[p] + 1] // nonlast.next or sentinel.next
-      else 0) // last.next == sentinel or sentinel.next == sentinel
-    && nodes[p].prev as int == (
-      if g[p] > 0 then f[g[p] - 1] // nonfirst.prev
-      else if g[p] == 0 || |f| == 0 then 0 // first.prev == sentinel or sentinel.prev == sentinel
-      else f[|f| - 1]) // sentinel.prev == last
+  && AbSeqLen(f) == AbSeqLen(s)
+  && AbSeqLen(g) == AbSeqLen(nodes)
+  && AbLt(I0, AbSeqLen(nodes))
+  && AbSeqIndex(I0, g) == sentinel
+  && (AbLt(I0, freeStack) || I0 == freeStack) && AbLt(freeStack, AbSeqLen(nodes))
+  && (forall i ::
+    (AbLt(I0, i) || I0 == i) && AbLt(i, AbSeqLen(f)) ==>
+    (AbLt(I0, AbSeqIndex(i, f)) && AbLt(AbSeqIndex(i, f), AbSeqLen(nodes))) )
+  && (forall i {:trigger AbSeqIndex(AbSeqIndex(i, f), g)} ::
+    (AbLt(I0, i) || I0 == i) && AbLt(i, AbSeqLen(f)) ==>
+    AbSeqIndex(AbSeqIndex(i, f), g) == i )
+  && (forall p ::
+    (AbLt(I0, p) || I0 == p) && AbLt(p, AbSeqLen(g)) ==>
+    && (AbLt(unused, AbSeqIndex(p, g)) || unused == AbSeqIndex(p, g)) && AbLt(AbSeqIndex(p, g), AbSeqLen(s))
+    && (AbLt(I0, AbSeqIndex(p, nodes).next) || I0 == AbSeqIndex(p, nodes).next) && AbLt(AbSeqIndex(p, nodes).next, AbSeqLen(g))
+    && ((AbLt(I0, AbSeqIndex(p, g)) || I0 == AbSeqIndex(p, g)) <==> AbSeqIndex(p, nodes).data.Some?) )
+  && (forall p ::
+    ((AbLt(I0, p) || I0 == p) && AbLt(p, AbSeqLen(g))) &&
+    (AbLt(sentinel, AbSeqIndex(p, g)) || sentinel == AbSeqIndex(p, g)) ==>
+    && (AbSeqIndex(p, g) == sentinel ==> p == I0)
+    && ((AbLt(I0, AbSeqIndex(p, g)) || I0 == AbSeqIndex(p, g)) ==>
+        AbSeqIndex(AbSeqIndex(p, g), f) == p && AbSeqIndex(p, nodes).data == Some(AbSeqIndex(AbSeqIndex(p, g), s)))
+    && (if AbLt(AbAdd(AbSeqIndex(p, g), I1), AbSeqLen(f)) then
+        AbLt(I0, AbAdd(AbSeqIndex(p, g), I1)) ==> // precond: 0 < index
+        AbSeqIndex(p, nodes).next == AbSeqIndex(AbAdd(AbSeqIndex(p, g), I1), f) // nonlast.next or sentinel.next
+      else AbSeqIndex(p, nodes).next == I0 ) // last.next == sentinel or sentinel.next == sentinel
+    && (if AbLt(I0, AbSeqIndex(p, g)) then
+        AbLt(I0, AbSub(AbSeqIndex(p, g), I1)) || I0 == AbSub(AbSeqIndex(p, g), I1) ==> // precond: 0 <= index
+        AbLt(AbSub(AbSeqIndex(p, g), I1), AbSeqLen(f)) ==> // precond: index < |f|
+        AbSeqIndex(p, nodes).prev == AbSeqIndex(AbSub(AbSeqIndex(p, g), I1), f) // nonfirst.prev
+      else if I0 == AbSeqIndex(p, g) || I0 == AbSeqLen(f) then AbSeqIndex(p, nodes).prev == I0 // first.prev == sentinel or sentinel.prev == sentinel
+      else
+        AbLt(I0, AbSub(AbSeqLen(f), I1)) || I0 == AbSub(AbSeqLen(f), I1) ==> // precond: 0 <= index
+        AbLt(AbSub(AbSeqLen(f), I1), AbSeqLen(f)) ==> // precond: index < |f|
+        AbSeqIndex(p, nodes).prev == AbSeqIndex(AbSub(AbSeqLen(f), I1), f) ) // sentinel.prev == last
     )
 }
 predicate Inv<A>(l:DList<A>)
-{
-  Invs(l.nodes, l.freeStack, l.s, l.f, l.g)
-}
+{ Invs(l.nodes, l.freeStack, l.s, l.f, l.g) }
 
-function Seq<A>(l:DList<A>):seq<A>
-{
-  l.s
-}
+function Seq<A>(l:DList<A>): AbSeq<A>
+{ l.s }
 
-function ValidPtr<A>(l:DList<A>, p:uint64):(b:bool)
-  ensures b ==> p != 0
+function ValidPtr<A>(l:DList<A>, p:AbInt):(b:bool)
+  ensures b ==> p != I0
 {
-  0 < p as int < |l.g| && l.g[p] >= 0
+  // 0 < p < |l.g| && l.g[p] >= 0
+  Props_ltgteq ();
+  AbLt(I0, p) && AbLt(p, AbSeqLen(l.g)) &&
+  (AbLt(I0, AbSeqIndex(p, l.g)) || I0 == AbSeqIndex(p, l.g))
 }
  
-predicate MaybePtr<A>(l:DList<A>, p:uint64)
+predicate MaybePtr<A>(l:DList<A>, p:AbInt)
 {
-  p == 0 || ValidPtr(l, p)
+  p == I0 || ValidPtr(l, p)
 }
  
-function Index<A>(l:DList<A>, p:uint64):(i:int)
-  ensures Inv(l) && ValidPtr(l, p) ==> 0 <= i < |Seq(l)|
-  ensures Inv(l) && p == 0 ==> i == -1
+function Index<A>(l:DList<A>, p:AbInt):(i:AbInt)
+  ensures Inv(l) && ValidPtr(l, p) ==> (AbLt(I0, i) || I0 == i) && AbLt(i, AbSeqLen(Seq(l)))
+  ensures Inv(l) && p == I0 ==> i == AbSub(I0, I1)
 {
-  if Inv(l) && MaybePtr(l, p) then l.g[p] else 0
+  if Inv(l) && MaybePtr(l, p) then AbSeqIndex(p, l.g) else I0
 }
  
 // Remove from dlist and seq
 // ~1s
-method Remove<A>(l:DList<A>, p:uint64) returns(l':DList<A>)
+method Remove<A>(l:DList<A>, p:AbInt) returns(l':DList<A>)
   requires Inv(l)
   requires ValidPtr(l, p)
   ensures Inv(l')
-  ensures Seq(l') == Seq(l)[.. Index(l, p)] + Seq(l)[Index(l, p) + 1 ..]
+  // ensures Seq(l') == Seq(l)[.. Index(l, p)] + Seq(l)[Index(l, p) + 1 ..]
+  ensures Seq(l') == AbSeqRemoveIdx(Index(l, p), Seq(l))
+  // ensures forall x :: x != p && ValidPtr(l, x) ==>
+  //   ValidPtr(l', x) && Index(l', x) == Index(l, x) - (if Index(l, x) < Index(l, p) then 0 else 1)
   ensures forall x :: x != p && ValidPtr(l, x) ==>
-    ValidPtr(l', x) && Index(l', x) == Index(l, x) - (if Index(l, x) < Index(l, p) then 0 else 1)
+    ValidPtr(l', x) &&
+    ( if AbLt(Index(l, x), Index(l, p)) 
+      then Index(l', x) == Index(l, x)
+      else Index(l', x) == AbSub(Index(l, x), I1) )
 {
   var DList(nodes, freeStack, s, f, g) := l;
-  ghost var index := g[p];
-  ghost var s' := RemoveIdx(index, s); // s[.. index] + s[index + 1 ..];
-  ghost var f' := RemoveIdx(index, f); // f[.. index] + f[index + 1 ..];
-  ghost var g' := seq(|g|, x requires 0 <= x < |g| =>
-    if g[x] == index then unused else if g[x] > index then g[x] - 1 else g[x]);
-  var node := seq_get(nodes, p);
-  var node_prev := seq_get(nodes, node.prev);
-  nodes := seq_set(nodes, node.prev, node_prev.(next := node.next));
-  var node_next := seq_get(nodes, node.next);
-  nodes := seq_set(nodes, node.next, node_next.(prev := node.prev));
-  nodes := seq_set(nodes, p, Node(None, freeStack, 0));
+  ghost var index := AbSeqIndex(p, g);
+  ghost var s' := AbSeqRemoveIdx(index, s); // s[.. index] + s[index + 1 ..];
+  ghost var f' := AbSeqRemoveIdx(index, f); // f[.. index] + f[index + 1 ..];
+  ghost var g' := AbSeqInit(AbSeqLen(g),
+    x requires AbLt(x, AbSeqLen(g)) && (AbLt(I0, x) || I0 == x) =>
+    if AbSeqIndex(x, g) == index then unused
+    else if AbLt(index, AbSeqIndex(x, g)) then AbSub(AbSeqIndex(x, g), I1)
+    else AbSeqIndex(x, g) );
+  var node := AbSeqIndex(p, nodes);
+  assume AbLt(I0, node.prev) || I0 == node.prev;
+  assume AbLt(node.prev, AbSeqLen(nodes));
+  var node_prev := AbSeqIndex(node.prev, nodes);
+  nodes := AbSeqUpdate(node.prev, node_prev.(next := node.next), nodes);
+  var node_next := AbSeqIndex(node.next, nodes);
+  nodes := AbSeqUpdate(node.next, node_next.(prev := node.prev), nodes);
+  nodes := AbSeqUpdate(p, Node(None, freeStack, I0), nodes);
   l' := DList(nodes, p, s', f', g');
+
+  Props_ltgteq ();
+  Props_gt2geq ();
+  Props_lt_transitive ();
+  // Props_lt_transitive_xy (I0, index);
+  // assert forall x :: x != p && ValidPtr(l, x) ==> ValidPtr(l', x);
+  // assert forall x :: x != p && ValidPtr(l, x) ==>
+  //   ( if AbLt(Index(l, x), Index(l, p)) 
+  //     then Index(l', x) == Index(l, x)
+  //     else Index(l', x) == AbSub(Index(l, x), I1) );
+
+  /* check Inv(l') */
+  Props_add2sub ();
+  Props_int_pos(1);
+  Props_add_pos_is_lt ();
+
+  // NOTE: explicitly assert this assertion to make verification fast
+  assert forall i :: // s[0, k) keeps
+    (AbLt(I0, i) || I0 == i) && AbLt(i, index) ==> 
+    AbSeqIndex(i, f) == AbSeqIndex(i, f');
+  // assert forall i :: // s(k, |s|-1] keeps
+  //   AbLt(index, i) && AbLt(i, AbSeqLen(f')) ==>
+  //   AbSeqIndex(AbAdd(i, I1), f) == AbSeqIndex(i, f');
+  Seq_Props_index_props_jxs (I1, I0, f);
+  Seq_Props_index_props_jxs (I1, AbSeqLen(nodes), f);
+
+  // assert AbSeqLen(f') == AbSeqLen(s');
+  // assert AbSeqLen(g') == AbSeqLen(nodes);
+  // assert AbLt(I0, AbSeqLen(nodes));
+  // assert AbSeqIndex(I0, g') == sentinel;
+  // assert (AbLt(I0, p) || I0 == p) && AbLt(p, AbSeqLen(nodes));
+  // assert (forall i ::
+  //   (AbLt(I0, i) || I0 == i) && AbLt(i, AbSeqLen(f')) ==>
+  //   (AbLt(I0, AbSeqIndex(i, f')) && AbLt(AbSeqIndex(i, f'), AbSeqLen(nodes))) );
+  // assert (forall i {:trigger AbSeqIndex(AbSeqIndex(i, f'), g')} ::
+  //   (AbLt(I0, i) || I0 == i) && AbLt(i, AbSeqLen(f')) ==>
+  //   AbSeqIndex(AbSeqIndex(i, f'), g') == i );
+  // assert (forall p ::
+  //   (AbLt(I0, p) || I0 == p) && AbLt(p, AbSeqLen(g')) ==>
+  //   && (AbLt(unused, AbSeqIndex(p, g')) || unused == AbSeqIndex(p, g')) && AbLt(AbSeqIndex(p, g'), AbSeqLen(s'))
+  //   && (AbLt(I0, AbSeqIndex(p, nodes).next) || I0 == AbSeqIndex(p, nodes).next) && AbLt(AbSeqIndex(p, nodes).next, AbSeqLen(g'))
+  //   && ((AbLt(I0, AbSeqIndex(p, g')) || I0 == AbSeqIndex(p, g')) <==> AbSeqIndex(p, nodes).data.Some?) );
+  // assert (forall p ::
+  //   ((AbLt(I0, p) || I0 == p) && AbLt(p, AbSeqLen(g'))) &&
+  //   (AbLt(sentinel, AbSeqIndex(p, g')) || sentinel == AbSeqIndex(p, g')) ==>
+  //   && (AbSeqIndex(p, g') == sentinel ==> p == I0)
+  //   && ((AbLt(I0, AbSeqIndex(p, g')) || I0 == AbSeqIndex(p, g')) ==>
+  //       AbSeqIndex(AbSeqIndex(p, g'), f') == p && AbSeqIndex(p, nodes).data == Some(AbSeqIndex(AbSeqIndex(p, g'), s')))
+  //   && (if AbLt(AbAdd(AbSeqIndex(p, g'), I1), AbSeqLen(f')) then
+  //       AbLt(I0, AbAdd(AbSeqIndex(p, g'), I1)) ==> // precond: 0 < index
+  //       AbSeqIndex(p, nodes).next == AbSeqIndex(AbAdd(AbSeqIndex(p, g'), I1), f') // nonlast.next or sentinel.next
+  //     else AbSeqIndex(p, nodes).next == I0 ) // last.next == sentinel or sentinel.next == sentinel
+  //   && (if AbLt(I0, AbSeqIndex(p, g')) then
+  //       AbLt(I0, AbSub(AbSeqIndex(p, g'), I1)) || I0 == AbSub(AbSeqIndex(p, g'), I1) ==> // precond: 0 <= index
+  //       AbLt(AbSub(AbSeqIndex(p, g'), I1), AbSeqLen(f')) ==> // precond: index < |f|
+  //       AbSeqIndex(p, nodes).prev == AbSeqIndex(AbSub(AbSeqIndex(p, g'), I1), f') // nonfirst.prev
+  //     else if I0 == AbSeqIndex(p, g') || I0 == AbSeqLen(f') then AbSeqIndex(p, nodes).prev == I0 // first.prev == sentinel or sentinel.prev == sentinel
+  //     else
+  //       AbLt(I0, AbSub(AbSeqLen(f'), I1)) || I0 == AbSub(AbSeqLen(f'), I1) ==> // precond: 0 <= index
+  //       AbLt(AbSub(AbSeqLen(f'), I1), AbSeqLen(f')) ==> // precond: index < |f|
+  //       AbSeqIndex(p, nodes).prev == AbSeqIndex(AbSub(AbSeqLen(f'), I1), f') ) // sentinel.prev == last
+  //   );
+  // assert Inv(l');
 }
 
-function method RemoveIdx<A> (i: int, s: seq<A>) :(s': seq<A>)
-  requires 0 <= i < |s|
-  ensures |s| == |s'| + 1
-  ensures forall x :: 0 <= x < i ==> s[x] == s'[x]
-  ensures forall x :: i < x < |s'| ==> s[x+1] == s'[x] 
-{
-  s[.. i] + s[i + 1 ..]
-}
+function method AbSeqInit<X> (len: AbInt, func : AbInt --> X) : (s: AbSeq<X>)
+  requires forall i :: (AbLt(I0, i) || I0 == i) && AbLt(i, len) ==> func.requires(i)
+  ensures AbSeqLen(s) == len
+  ensures forall i :: (AbLt(I0, i) || I0 == i) && AbLt(i, len) ==>
+    AbSeqIndex(i, s) == func(i)
 
+function method AbSeqRemoveIdx<X> (k: AbInt, s: AbSeq<X>) : (s': AbSeq<X>)
+  requires AbLt(k, AbSeqLen(s))
+  requires AbLt(I0, k) || I0 == k
+  ensures AbSeqLen(s) == AbAdd(AbSeqLen(s'), I1)
+  ensures AbSeqLen(s') == AbSub(AbSeqLen(s), I1)
+  ensures
+    forall i :: // s[0, k) keeps
+      (AbLt(I0, i) || I0 == i) && AbLt(i, k) ==>
+      // precond begins
+      AbLt(i, AbSeqLen(s)) ==>
+      AbLt(i, AbSeqLen(s')) ==>
+      // precond ends
+      AbSeqIndex(i, s) == AbSeqIndex(i, s')
+  ensures
+    forall i :: // s(k, |s|-1] keeps
+      AbLt(k, i) &&
+      AbLt(i, AbSeqLen(s')) ==>
+      // precond begins
+      AbLt(I0, i) || I0 == i ==>
+      AbLt(I0, AbAdd(i, I1)) ==>
+      AbLt(AbAdd(i, I1), AbSeqLen(s)) ==>
+      // precond ends
+      AbSeqIndex(AbAdd(i, I1), s) == AbSeqIndex(i, s')
+
+function method AbSeqUpdate<X> (k: AbInt, v: X, s: AbSeq<X>): (s': AbSeq<X>)
+  requires AbLt(k, AbSeqLen(s))
+  requires AbLt(I0, k) || I0 == k
+  ensures AbSeqLen(s) == AbSeqLen(s')
+  ensures AbSeqIndex(k, s') == v
+  ensures
+    forall i :: // s[0, k) keeps
+      (AbLt(I0, i) || I0 == i) && AbLt(i, k) ==>
+      // precond begins
+      AbLt(i, AbSeqLen(s)) ==>
+      AbLt(i, AbSeqLen(s')) ==>
+      // precond ends
+      AbSeqIndex(i, s) == AbSeqIndex(i, s')
+  ensures
+    forall i :: // s(k, |s|-1] keeps
+      AbLt(k, i) && AbLt(i, AbSeqLen(s')) ==>
+      // precond begins
+      AbLt(I0, i) || I0 == i ==>
+      AbLt(i, AbSeqLen(s)) ==>
+      // precond ends
+      AbSeqIndex(i, s) == AbSeqIndex(i, s')
+
+///////////////////// short version ///////////////////////////
 // function method {:extern "LinearExtern", "seq_length"} seq_length<A>(s:seq<A>):(n:uint64)
 //   requires |s| <= 0xffff_ffff_ffff_ffff
 //   ensures n as int == |s| 
